Finished implementing the method InsertBST in BST file. The program compiles with 0 errors and runs correctly.

BST.dfy
@@ -70,6 +70,152 @@ method BuildBST(q: seq<int>) returns (t: Tree)
 method InsertBST(t0: Tree, x: int) returns (t: Tree)
 	requires BST(t0) && x !in NumbersInTree(t0)
 	ensures BST(t) && NumbersInTree(t) == NumbersInTree(t0)+{x}
+{
+	match t0 {
+		case Empty => t := Node(x, Empty, Empty);
+		case Node(n',nt1,nt2) => 
+			if(x < n')
+			{
+				LemmaBinarySearchSubtree(n',nt1,nt2);
+				var tLeft := InsertBST(nt1, x);
+				t := Node(n', tLeft, nt2);
+				L_BST(n', nt1, nt2);
+				/*
+				assert BST(t0);
+				assert greaterThanTree(nt1, n');
+				//==>
+				assert greaterThanTree(tLeft, n');
+				assert smallerThanTree(nt2, n');
+				*/
+				//L(n', tLeft, nt2);
+				L_greater(nt1, n', x, tLeft);
+
+				assert BST(t);
+			}
+			else
+			{
+				
+				LemmaBinarySearchSubtree(n',nt1,nt2);
+				var tRight:Tree := InsertBST(nt2, x);
+				t := Node(n', nt1, tRight);
+				L_BST(n', nt1, nt2);
+				
+				/*
+				assert BST(t0);
+				assert greaterThanTree(nt1, n');
+				
+				assert smallerThanTree(nt2, n');
+				assert n' < x;
+				assert NumbersInTree(tRight) == NumbersInTree(nt2)+{x};
+				//==>
+				assert greaterThanTree(nt1, n');
+				*/
+				//assert smallerThanTree(tRight, n');
+				
+				L_smaller(nt2, n', x, tRight);
+
+				assert NumbersInTree(t) == NumbersInTree(t0)+{x};
+
+				assert BST(t);
+				
+			}
+	}
+}
+/*
+predicate tree_NoDuplicates(t:Tree)
+{
+	NoDuplicates(Inorder(t))
+}
+*/
+lemma L3(t1:Tree, t2:Tree, x:int)
+	requires NumbersInTree(t1) == NumbersInTree(t2)+{x}
+	ensures forall i:: 0 <= i < |Inorder(t1)| ==> Inorder(t1)[i] in Inorder(t2) || Inorder(t1)[i] == x
+	ensures forall i:: 0 <= i < |Inorder(t2)| ==> Inorder(t2)[i] in Inorder(t1)
+{
+	var q1 := Inorder(t1);
+	var q2 := Inorder(t2);
+
+	assert NumbersInTree(t1) == NumbersInTree(t2)+{x};
+	//==>
+	assert NumbersInSequence(q1) == NumbersInTree(t2)+{x};
+	//==>
+	assert forall i:: 0 <= i < |q1| ==> q1[i] in NumbersInTree(t1);
+	assert forall i:: 0 <= i < |q2| ==> q2[i] in NumbersInTree(t1);
+	//==>
+	assert forall i:: 0 <= i < |q2| ==> q2[i] in q1;
+	assert forall i:: 0 <= i < |q1| ==> q1[i] in q2 || q1[i] == x;
+}
+
+
+lemma L_smaller(nt2:Tree, n':int, x:int, tRight:Tree)
+	requires smallerThanTree(nt2, n')
+	requires n' < x
+	requires NumbersInTree(tRight) == NumbersInTree(nt2)+{x}
+	ensures smallerThanTree(tRight, n')
+
+{
+	
+	L3(tRight, nt2, x);
+	//==>
+	assert forall i:: 0 <= i < |Inorder(tRight)| ==> n' < Inorder(tRight)[i];
+	//==>
+	assert smallerThanTree(tRight, n');
+}
+
+lemma L_greater(nt1:Tree, n':int, x:int, tLeft:Tree)
+	requires greaterThanTree(nt1, n')
+	requires x < n'
+	requires NumbersInTree(tLeft) == NumbersInTree(nt1)+{x}
+	ensures greaterThanTree(tLeft, n')
+{
+	L3(tLeft, nt1, x);
+	//==>
+	assert forall i:: 0 <= i < |Inorder(tLeft)| ==> Inorder(tLeft)[i] < n';
+	//==>
+	assert greaterThanTree(tLeft, n');
+}
+/*
+lemma L_Ascending(q:seq<int>, x:int)
+	requires Ascending(q+[x])
+	ensures forall i:: 0 <= i < |q| ==> q[i] < x
+*/
+
+lemma L_BST(n: int, left: Tree, right: Tree)
+	requires BST(Node(n, left, right))
+	ensures greaterThanTree(left, n)
+	ensures smallerThanTree(right, n)
+{
+	assert Ascending(Inorder(Node(n, left, right)));
+	var qleft, qright := Inorder(left), Inorder(right);
+	var q1 := qleft+[n]+qright;
+	var q2 := qleft+[n];
+	var q3 := [n]+qright;
+	LemmaAscendingSubsequence(q1, q2, 0);
+	LemmaAscendingSubsequence(q1, q3, |q2|-1);
+	assert q2[|q2|-1] == n;
+
+	//==>
+
+	assert greaterThanTree(left, n);
+	assert smallerThanTree(right, n);
+}
+
+predicate smallerThanTree(t:Tree, x:int)
+{
+	forall i:: 0 <= i < |Inorder(t)| ==> x < Inorder(t)[i]
+}
+
+predicate greaterThanTree(t:Tree, x:int)
+{
+	forall i:: 0 <= i < |Inorder(t)| ==> x > Inorder(t)[i]
+}
+
+lemma L(n: int, left: Tree, right: Tree)
+	requires BST(left) && BST(right)
+	requires forall i:: 0 <= i < |Inorder(left)| ==> n > Inorder(left)[i]
+	requires forall i:: 0 <= i < |Inorder(right)| ==> n < Inorder(right)[i]
+	ensures BST(Node(n, left, right))
+{}
 
 lemma	LemmaBinarySearchSubtree(n: int, left: Tree, right: Tree)
 	requires BST(Node(n, left, right))
